theories/Mon/sprop/Monoid.v
@@ -80,7 +80,7 @@ Section MonoidExamples.
   Program Definition overwriteMonoid (X:Type) : monoid :=
     @mkMonoid { f : X -> X ≫ s∃ (m: optionMonoid X), forall x, Some (f x) ≡ m⋅(Some x)}
               (exist _ id _)
-              (fun f g => exist _ (Spr1 f \o Spr1 g) _) _ _ _.
+              (fun f g => exist _ (proj1_sig f \o proj1_sig g) _) _ _ _.
   Next Obligation. exists None. move=> ? //. Qed.
   Next Obligation.
     (* move: f g => [? [mf Hf]] [? [mg Hg]]. *)
@@ -151,7 +151,7 @@ Section ActionExamples.
 
   Program Definition overwriteAction (X:Type)
     : monoid_action (overwriteMonoid X) :=
-    @mkAction _ X (fun f x => Spr1 f x) _ _.
+    @mkAction _ X (fun f x => proj1_sig f x) _ _.
 End ActionExamples.
 
 Section MonoidStrictification.
@@ -167,7 +167,7 @@ Section MonoidStrictification.
   Qed.
 
   Program Definition smult (sm1 sm2 : SM) : SM :=
-    exist _ (Spr1 sm1 \o Spr1 sm2) _.
+    exist _ (proj1_sig sm1 \o proj1_sig sm2) _.
   Next Obligation.
     move:sm1 sm2=> [? [m1 H1]] [? [m2 H2]].
     exists (m1 ⋅ m2) ; move=> m /=.
@@ -179,13 +179,13 @@ Section MonoidStrictification.
   Program Definition embed (m:M) : SM := exist _ (monoid_mult m) _.
   Next Obligation. exists m ; move=> ? //. Qed.
 
-  Definition project (sm : SM) : M := Spr1 sm (e M).
+  Definition project (sm : SM) : M := proj1_sig sm (e M).
 
   Lemma embed_project_id : forall m, project (embed m) = m.
   Proof. intro. cbv. rewrite monoid_law2 //. Qed.
 
   Lemma sig_sEq : forall (A : Type) (P : A -> Prop) (mx my : {x : A ≫ P x}),
-       Spr1 mx ≡ Spr1 my -> mx ≡ my.
+       proj1_sig mx ≡ proj1_sig my -> mx ≡ my.
   Proof.
     intros A P [mx ?] [my ?] H. simpl in H.
     induction H. compute. f_equal. apply ax_proof_irrel.
@@ -195,7 +195,7 @@ Section MonoidStrictification.
   Lemma project_embed_id : forall sm, embed (project sm) ≡ sm.
   Proof.
     intro sm. apply sig_sEq ; funext m0.
-    cbv. move: (Spr2 sm) => [m Hm].
+    cbv. move: (proj2_sig sm) => [m Hm].
     pose (H0 := Hm m0).
     apply sEq_sym in H0.
     unshelve eapply (sEq_trans _ H0).
