theories/Relational/GenericRulesSimple.v
@@ -17,7 +17,7 @@ Set Universe Polymorphism.
 (*   Context (η : natTrans Jprod W) (σ := point_to_homomorphism Jprod rmW η). *)
 
 (*   Definition mod_semantic_judgement {A1 A2} c1 c2 w := *)
-(*     Spr1 (σ ⟨A1,A2⟩) ⟨c1,c2⟩ ≤ w. *)
+(*     proj1_sig (σ ⟨A1,A2⟩) ⟨c1,c2⟩ ≤ w. *)
 
 (*   Notation "⊨ c1 ≈ c2 [{ w }]" := (@mod_semantic_judgement _ _ c1 c2 w). *)
 
@@ -28,7 +28,7 @@ Set Universe Polymorphism.
 (*   Proof. move=> ? ? ; rewrite /mod_semantic_judgement ; estransitivity ; eassumption. Qed. *)
 
 (*   Lemma ret_rule {A B} {a : A} {b : B} : *)
-(*     ⊨ ret a ≈ ret b [{ Spr1 (η ⟨A,B⟩) ⟨a,b⟩ }]. *)
+(*     ⊨ ret a ≈ ret b [{ proj1_sig (η ⟨A,B⟩) ⟨a,b⟩ }]. *)
 (*   Proof. *)
 (*     rewrite /mod_semantic_judgement. *)
 (*     move: (point_to_homomorphism_to_point Jprod rmW η ⟨A, B⟩ ⟨a,b⟩) => /= ->. *)
@@ -37,7 +37,7 @@ Set Universe Polymorphism.
 
 (*   Definition bindW {A1 A2 B1 B2} *)
 (*              (f1 : A1 -> M1 B1) (f2 : A2 -> M2 B2) (w : dfst (W ⟨A1,A2⟩)) := *)
-(*     Spr1 (rm_bind rmW (to_prod f1 f2)) w. *)
+(*     proj1_sig (rm_bind rmW (to_prod f1 f2)) w. *)
 
 (*   Lemma bind_act_rule {A1 A2 B1 B2} *)
 (*         {m1 : M1 A1} {m2 : M2 A2} {w} : *)
@@ -48,7 +48,7 @@ Set Universe Polymorphism.
 (*     move=> H f1 f2. *)
 (*     pose (rm_homo _ rmW σ (to_prod f1 f2) ⟨m1, m2⟩) as t. *)
 (*     move: t => /= ->. unfold bindW. *)
-(*     apply (Spr2 (rm_bind rmW (to_prod f1 f2)))=> //=. *)
+(*     apply (proj2_sig (rm_bind rmW (to_prod f1 f2)))=> //=. *)
 (*   Qed. *)
 
 (*   Lemma if_rule {A1 A2} {m1: M1 A1} {m2 : M2 A2} {w w'} (b:bool) : *)
@@ -74,7 +74,7 @@ Section RelationalProgramLogicFromRelativeMonadZero.
   Context (W : RelationalSpecMonad0)
           (θ : RelationalLaxEffectObservation0 M1 M2 W).
 
-  Definition semantic_judgement A1 A2 c1 c2 w := Spr1 (θ ⟨A1,A2⟩) ⟨c1,c2⟩ ≤ w.
+  Definition semantic_judgement A1 A2 c1 c2 w := proj1_sig (θ ⟨A1,A2⟩) ⟨c1,c2⟩ ≤ w.
   Notation "⊨ c1 ≈ c2 [{ w }]" := (semantic_judgement _ _ c1 c2 w).
 
   Check (fun A B (c1 : M1 A) (c2: M2 B) w => ⊨ c1 ≈ c2 [{ w }] ).
@@ -131,7 +131,7 @@ Section GoingPractical.
   Context (W : RelationalSpecMonad0) (θ : RelationalLaxEffectObservation0 M1 M2 W).
 
   Lemma gp_ret_rule {A B a b w} :
-    Spr1 (ord_relmon_unit W ⟨A , B⟩) ⟨a,b⟩ ≤ w ->
+    proj1_sig (ord_relmon_unit W ⟨A , B⟩) ⟨a,b⟩ ≤ w ->
     θ ⊨ ret a ≈ ret b [{ w }].
   Proof. apply weaken_rule2 ; apply ret_rule2. Qed.
 
@@ -141,7 +141,7 @@ Section GoingPractical.
         {f1 : A1 -> M1 B1} {f2 : A2 -> M2 B2}
         {wf : OrdCat⦅Jprod ⟨A1,A2⟩ ; W ⟨B1, B2⟩⦆} {w} :
     θ ⊨ m1 ≈ m2 [{ wm }] ->
-    (forall a1 a2, θ ⊨ f1 a1 ≈ f2 a2 [{ Spr1 wf ⟨a1, a2⟩ }]) ->
+    (forall a1 a2, θ ⊨ f1 a1 ≈ f2 a2 [{ proj1_sig wf ⟨a1, a2⟩ }]) ->
     wm ≫= wf ≤ w ->
     θ ⊨ bind m1 f1 ≈ bind m2 f2 [{ w }].
   Proof. move=> ? ? ; apply weaken_rule2 ; apply seq_rule=> //. Qed.
@@ -258,11 +258,11 @@ Section GoingPractical.
   (*    a safer approach would consist in defining an inductive for ⊢) *)
   (*    assuming the bimodules rules, so not achieving much *) *)
   (* Lemma to_spec {A1 A2} {m1 : M1 A1} {m2 : M2 A2} {w} : *)
-  (*   Spr1 (θ ⟨_,_⟩) ⟨m1, m2⟩ ≤ w -> θ ⊨ m1 ≈ m2 [{ w }]. *)
+  (*   proj1_sig (θ ⟨_,_⟩) ⟨m1, m2⟩ ≤ w -> θ ⊨ m1 ≈ m2 [{ w }]. *)
   (* Proof. *)
   (*   enough (m1 = skip ;; m1) as ->. *)
   (*   enough (m2 = skip ;; m2) as ->. *)
-  (*   enough (Spr1 (θ ⟨_,_⟩) ⟨skip ;; m1, skip ;; m2⟩ = act (fun=> m1) (fun=> m2) (Spr1 (rmon_unit W ⟨_,_⟩) ⟨tt,tt⟩)) as ->. *)
+  (*   enough (proj1_sig (θ ⟨_,_⟩) ⟨skip ;; m1, skip ;; m2⟩ = act (fun=> m1) (fun=> m2) (proj1_sig (rmon_unit W ⟨_,_⟩) ⟨tt,tt⟩)) as ->. *)
   (*   apply cont_to_spec. *)
   (*   rewrite /skip ; apply ret_rule2. *)
   (*   move: (rmm_law2 _ _ _ _ θ _ _ (to_prod (fun=> m1) (fun=> m2)) ⟨skip,skip⟩) *)
